add elaboration from type assignment system to bidirectional system

src-lite/bidir/elaboration.v
@@ -9,14 +9,13 @@ Definition to_k (bk : bkind) : kind :=
   end
 .
 
-
-Inductive wf_context_elab : bcontext → context → Prop :=
-| wfe_nil : wf_context_elab bctx_nil ctx_nil
+Inductive wf_bcontext_elab : bcontext → context → Prop :=
+| wfe_nil : wf_bcontext_elab bctx_nil ctx_nil
 | wfe_cons : forall Γ' Γ x A' A k
-  , wf_context_elab Γ' Γ
+  , wf_bcontext_elab Γ' Γ
   → x `notin` bctx_dom Γ'
   -> busub_elab Γ' A' A' d_infer ⧼k⧽' Γ A A ⧼(to_k k)⧽
-  -> wf_context_elab (Γ' ,' x : A') (Γ, x : A)
+  -> wf_bcontext_elab (Γ' ,' x : A') (Γ, x : A)
 with infer_app_elab
   : bcontext -> bexpr -> bexpr -> bexpr
   -> expr → expr → Prop :=
@@ -51,16 +50,16 @@ with busub_elab
   : bcontext → bexpr → bexpr → dir  → bexpr
   →  context →  expr →  expr → expr → Prop :=
 | bse_var : forall Γ Γ' x A A'
-  , wf_context_elab Γ' Γ -> in_bctx x A' Γ' → in_ctx x A Γ
+  , wf_bcontext_elab Γ' Γ -> in_bctx x A' Γ' → in_ctx x A Γ
   -> busub_elab Γ' `'x `'x d_infer A' Γ `x `x A
 | bse_lit : forall Γ' Γ n
-  , wf_context_elab Γ' Γ
+  , wf_bcontext_elab Γ' Γ
   -> busub_elab Γ' (be_num n) (be_num n) d_infer be_int Γ (e_num n) (e_num n) e_int
 | bse_star : forall Γ' Γ dir
-  , wf_context_elab Γ' Γ
+  , wf_bcontext_elab Γ' Γ
   -> busub_elab Γ' ⋆' ⋆' dir ◻' Γ ⋆ ⋆ ◻
 | bse_int : forall Γ' Γ
-  , wf_context_elab Γ' Γ
+  , wf_bcontext_elab Γ' Γ
   -> busub_elab Γ' be_int be_int d_infer ⋆' Γ e_int e_int ⋆
 | bse_bot : forall Γ' Γ A' A k
   , busub_elab Γ' A' A' d_infer ⧼k⧽' Γ A A ⧼(to_k k)⧽
@@ -153,3 +152,128 @@ with busub_elab
   -> busub_elab Γ' A' B' d_infer ⧼k⧽' Γ A B ⧼(to_k k)⧽
   -> busub_elab Γ' e1' e2' d_check B' Γ e1 e2 B
 .
+
+Definition to_bk (k : kind) : bkind :=
+  match k with
+  | k_star => bk_star
+  | k_box  => bk_box
+  end
+.
+
+Inductive wf_context_elab : context → bcontext → Prop :=
+| wf_nil : wf_context_elab ctx_nil bctx_nil
+| wf_cons : forall Γ x A k Γ' A'
+  , wf_context_elab Γ Γ'
+  -> x `notin` ctx_dom Γ
+  -> usub_elab Γ A A ⧼k⧽ Γ' A' A' ⧼(to_bk k)⧽'
+  -> wf_context_elab (Γ , x : A) (Γ' ,' x : A')
+with usub_elab
+  : context  → expr  → expr  → expr
+  → bcontext → bexpr → bexpr → bexpr → Prop :=
+| s_var : forall Γ x A Γ' A'
+  , wf_context_elab Γ Γ'
+  -> in_ctx x A Γ
+  -> usub_elab Γ `x `x A Γ' `'x `'x A'
+| s_lit : forall Γ n Γ'
+  , wf_context_elab Γ Γ'
+  → usub_elab Γ (e_num n) (e_num n) e_int Γ' (be_num n) (be_num n) be_int
+| s_star : forall Γ Γ'
+  , wf_context_elab Γ Γ'
+  → usub_elab Γ ⋆ ⋆ ◻ Γ' ⋆' ⋆' ◻'
+| s_int : forall Γ Γ'
+  , wf_context_elab Γ Γ'
+  -> usub_elab Γ e_int e_int ⋆ Γ' be_int be_int ⋆'
+| s_bot : forall Γ A1 A2 Γ' A1' A2' k
+  , usub_elab Γ A1 A2 ⧼k⧽ Γ' A1' A2' ⧼(to_bk k)⧽'
+  → usub_elab Γ A2 A1 ⧼k⧽ Γ' A2' A1' ⧼(to_bk k)⧽'
+  -> usub_elab Γ  (e_bot     A1 ) (e_bot     A2 ) A1
+              Γ' (be_bot ::' A1') (be_bot ::' A2') A1'
+| s_abs : forall L Γ Γ' A1 A1' e1 e1' B1 B1' A2 A2' e2 e2' B2 B2' k1 k2
+  , usub_elab Γ A1 A2 ⧼k1⧽ Γ' A1' A2' ⧼(to_bk k1)⧽'
+  → usub_elab Γ A2 A1 ⧼k1⧽ Γ' A2' A1' ⧼(to_bk k1)⧽'
+  → (forall x , x \notin L
+    → usub_elab (Γ , x : A1 ) (B1  ^`  x) (B2  ^`  x) ⧼k2⧽
+                (Γ','x : A1') (B1' ^`' x) (B2' ^`' x) ⧼(to_bk k2)⧽')
+  → (forall x , x \notin L
+    → usub_elab (Γ , x : A1 ) (B2  ^`  x) (B1  ^`  x) ⧼k2⧽
+                (Γ','x : A1') (B2' ^`' x) (B1' ^`' x) ⧼(to_bk k2)⧽')
+  → (forall x , x \notin L
+    → usub_elab (Γ , x : A1 ) (e1  ^`  x) (e2  ^`  x) (B1  ^`  x)
+                (Γ','x : A1') (e1' ^`' x) (e2' ^`' x) (B1' ^`' x))
+  → usub_elab Γ (λ_ A1, e1 : B1) (λ_ A2, e2 : B2) (e_pi A1 B1)
+              Γ' (be_abs e1' ::' be_pi A1' B1')
+                 (be_abs e1' ::' be_pi A2' B2') (be_pi A1' B1')
+| s_pi : forall L Γ Γ' A1 A1' B1 B1' A2 A2' B2 B2' k1 k2
+  , usub_elab Γ A1 A1 ⧼k1⧽ Γ' A1' A1' ⧼(to_bk k1)⧽'
+  -> usub_elab Γ A2 A1 ⧼k1⧽ Γ' A2' A1' ⧼(to_bk k1)⧽'
+  -> (forall x , x \notin  L
+    → usub_elab (Γ , x : A1 ) (B1  ^`  x) (B1  ^`  x) ⧼k2⧽
+                (Γ','x : A1') (B1' ^`' x) (B1' ^`' x) ⧼(to_bk k2)⧽')
+  -> (forall x , x \notin  L
+    → usub_elab (Γ , x : A2 ) (B1  ^`  x) (B2  ^`  x) ⧼k2⧽
+                (Γ','x : A2') (B1' ^`' x) (B2' ^`' x) ⧼(to_bk k2)⧽')
+  → usub_elab Γ  (e_pi  A1  B1 ) (e_pi  A2  B2 ) ⧼k2⧽
+              Γ' (be_pi A1' B1') (be_pi A2' B2') ⧼(to_bk k2)⧽'
+| s_app : forall Γ Γ' e1 e1' t t' e2 e2' A A' B B'
+  , mono_type t
+  -> usub_elab Γ t t A Γ' t' t' A'
+  -> usub_elab Γ e1 e2 (e_pi A B) Γ' e1' e2' (be_pi A' B')
+  -> usub_elab Γ  (e_app  e1  t ) (e_app  e2  t ) (B  ^^  t )
+              Γ' (be_app e1' t') (be_app e2' t') (B' ^^' t')
+| s_bind : forall L Γ Γ' A1 A1' e1 e1' B1 B1' A2 A2' e2 e2' B2 B2' k1 k2
+  , usub_elab Γ A1 A2 ⧼k1⧽ Γ' A1' A2' ⧼(to_bk k1)⧽'
+  → usub_elab Γ A2 A1 ⧼k1⧽ Γ' A2' A1' ⧼(to_bk k1)⧽'
+  → (forall x , x \notin L
+    → usub_elab (Γ , x : A1 ) (B1  ^`  x) (B2  ^`  x) ⧼k2⧽
+                (Γ','x : A1') (B1' ^`' x) (B2' ^`' x) ⧼(to_bk k2)⧽')
+  → (forall x , x \notin L
+    → usub_elab (Γ , x : A1 ) (B2  ^`  x) (B1  ^`  x) ⧼k2⧽
+                (Γ','x : A1') (B2' ^`' x) (B1' ^`' x) ⧼(to_bk k2)⧽')
+  → (forall x , x \notin L
+    → usub_elab (Γ , x : A1 ) (e1  ^`  x) (e2  ^`  x) (B1  ^`  x)
+                (Γ','x : A1') (e1' ^`' x) (e2' ^`' x) (B1' ^`' x))
+  → usub_elab Γ (Λ A1, e1 : B1) (Λ A2, e2 : B2) (e_all A1 B1)
+              Γ' (be_bind e1' ::' be_all A1' B1')
+                 (be_bind e1' ::' be_all A2' B2') (be_all A1' B1')
+| s_castup : forall Γ Γ' A1 A1' e1 e1' A2 A2' e2 e2' k B B'
+  , usub_elab Γ A1 A2 ⧼k⧽ Γ' A1' A2' ⧼(to_bk k)⧽'
+  → usub_elab Γ A2 A1 ⧼k⧽ Γ' A2' A1' ⧼(to_bk k)⧽'
+  → A1 ⟶ B
+  → A2 ⟶ B
+  → usub_elab Γ e1 e2 B Γ' e1' e2' B'
+  → usub_elab Γ  (e_castup A1 e1)       (e_castup A2 e2)      A1
+              Γ' (be_castup e1' ::' A1') (be_castup e2' ::' A2') A1'
+| s_castdn : forall Γ Γ' e1 e2 B k A e1' e2' A' B'
+  , usub_elab Γ B B ⧼k⧽ Γ' B' B' ⧼(to_bk k)⧽'
+  -> A ⟶ B
+  -> usub_elab Γ e1 e2 A Γ' e1' e2' A'
+  -> usub_elab Γ  (e_castdn  e1 ) (e_castdn  e2 ) B
+              Γ' (be_castdn e1') (be_castdn e2') B'
+| s_forall_l : forall L Γ Γ' A B C t A' B' C' t' k
+  , mono_type t
+  -> usub_elab Γ A A ⧼k⧽ Γ' A' A' ⧼(to_bk k)⧽'
+  -> usub_elab Γ t t A Γ' t' t' A'
+  -> usub_elab Γ (B ^^ t) C ⋆ Γ' (B' ^^' t') C' ⋆'
+  -> (forall x , x \notin  L
+    -> usub_elab (Γ , x : A) (B ^` x) (B ^` x) ⋆
+                (Γ','x : A') (B' ^`' x) (B' ^`' x) ⋆')
+  -> usub_elab Γ (e_all A B) C ⋆ Γ' (be_all A' B') C' ⋆'
+| s_forall_r : forall L Γ Γ' A B C A' B' C' k
+  , usub_elab Γ B B ⧼k⧽ Γ' B' B' ⧼(to_bk k)⧽'
+  -> usub_elab Γ A A ⋆ Γ' A' A' ⋆'
+  -> (forall x , x \notin L
+    -> usub_elab (Γ ,  x : B ) A  (C  ^`  x) ⋆
+                (Γ',' x : B') A' (C' ^`' x) ⋆')
+  -> usub_elab Γ A (e_all B C) ⋆ Γ' A' (be_all B' C') ⋆'
+| s_forall : forall L Γ Γ' A1 B A2 C A1' A2' B' C' k
+  , usub_elab Γ A1 A2 ⧼k⧽ Γ' A1' A2' ⧼(to_bk k)⧽'
+  → usub_elab Γ A2 A1 ⧼k⧽ Γ' A2' A1' ⧼(to_bk k)⧽'
+  -> (forall x , x \notin  L
+    -> usub_elab (Γ , x : A1 ) (B  ^`  x) (C  ^`  x) ⋆
+                (Γ','x : A1') (B' ^`' x) (C' ^`' x) ⋆')
+  -> usub_elab Γ  (e_all  A1  B ) (e_all  A2  C) ⋆
+              Γ' (be_all A1' B') (be_all A2' C') ⋆'
+| s_sub : forall Γ Γ' e1 e2 B A e1' e2' B' A' k
+  , usub_elab Γ e1 e2 A Γ' e1' e2' A'
+  -> usub_elab Γ A B ⧼k⧽ Γ' A' B' ⧼(to_bk k)⧽'
+  -> usub_elab Γ e1 e2 B Γ' (e1' ::' B') (e2' ::' B') B'.
